Weidenbach_Book/Watched_Literals/Watched_Literals_Transition_System_Restart.thy
@@ -1286,6 +1286,15 @@ lemma rtranclp_cdcl_twl_stgy_restart_with_leftovers_cdcl\<^sub>W_restart_stgy:
     by auto
   done
 *)
+
+definition partial_conclusive_TWL_run :: \<open>'v twl_st \<Rightarrow> (bool \<times> 'v twl_st) nres\<close> where
+  \<open>partial_conclusive_TWL_run S = SPEC(\<lambda>(b, T). \<exists>R1 R2 m.
+       cdcl_twl_stgy_restart\<^sup>*\<^sup>* (S, S, S, 0, 0, True) (R1, R2, T, m) \<and> (\<not>b \<longrightarrow> final_twl_state T))\<close>
+
+definition conclusive_TWL_run :: \<open>'v twl_st \<Rightarrow> 'v twl_st nres\<close> where
+  \<open>conclusive_TWL_run S = SPEC(\<lambda>T. (\<exists>R1 R2 m.
+       cdcl_twl_stgy_restart\<^sup>*\<^sup>* (S, S, S, 0, 0, True) (R1, R2, T, m) \<and> final_twl_state T))\<close>
+
 end
 
 end
